\section{Szabadtest-ábrák és a dinamika alaptétele}

\subsection{Ábrák}
\begin{figure}[H]
	\begin{minipage}[c]{.48\textwidth}
		\sztaone
	\end{minipage}
	\begin{minipage}{.48\textwidth}
		\begin{equation}
			\left[\dot{\pmb{I}}, \pmb{F}\right] 
			= \left[\dot{\pmb{\Pi}}_\text{S1}, \pmb{M}_\text{S1}\right]_\text{S}
		\end{equation}
		\begin{align}
			&x: m_1 {a_\text{S1}}_\text{x} 
			= C_\text{x} + D_\text{x} \\
			&y: m_1 {a_\text{S1}}_\text{y} 
			= C_\text{y} - G_1 + N_1 \\
			&z: {\theta_\text{S1}}_\text{z} \epsilon_1
			= D_\text{x} r_1
		\end{align}
	\end{minipage}
\end{figure}
\begin{figure}[H]
		\sztatr
		\begin{equation}
			\left[\dot{\pmb{I}}, \pmb{F}\right] 
			= \left[\dot{\pmb{\Pi}}_\text{S3}, \pmb{M}_\text{S3}\right]_\text{S}
		\end{equation}
		\begin{align}
			&x: m_3 {a_\text{S3}}_\text{x} 
			= -B_\text{x} + E_\text{x} \\
			&y: m_3 {a_\text{S3}}_\text{y} 
			= F_y - B_\text{y} + N_3 - G_3 \\
			&z: {\theta_\text{S3}}_\text{z} \epsilon_3
			= B_\text{x}\cdot l_3 \cos{\phi}
			- B_\text{y}\cdot l_3 \sin{\phi}
			+ E_\text{x} \cdot l_3
		\end{align}
\end{figure}

\newpage
\begin{figure}[H]
	\sztatwo
	\begin{equation}
		\left[\dot{\pmb{I}}, \pmb{F}\right] 
		= \left[\dot{\pmb{\Pi}}_\text{S2}, \pmb{M}_\text{S2}\right]_\text{S}
	\end{equation}
	\begin{align}
		&x: m_2 {a_\text{S2}}_\text{x} 
		= B_\text{x} - C_\text{x} \\
		&y: m_2 {a_\text{S2}}_\text{y} 
		= B_\text{y} - G_2 - C_\text{y} \\
		&z: {\theta_\text{S2}}_\text{z} \epsilon_2
		= -\left(
			B_\text{x}\cdot\frac{l_2}{2}\sin{\beta}
			+ C_\text{x}\cdot\frac{l_2}{2}\sin{\beta}
			+ B_\text{y}\cdot\frac{l_2}{2}\cos{\beta}
			+ C_\text{y}\cdot\frac{l_2}{2}\cos{\beta}
		\right)
	\end{align}
\end{figure}
